fstar/MLS.TreeDEM.PSK.fst
@@ -1,0 +1,141 @@
+module MLS.TreeDEM.PSK
+
+open MLS.Parser
+open MLS.Crypto
+//open Lib.IntTypes
+open Lib.ByteSequence
+module NT = MLS.NetworkTypes
+open MLS.Parser
+open MLS.Result
+
+#set-options "--fuel 0 --ifuel 0"
+
+type psk_type =
+  | PSKT_external
+  | PSKT_reinit
+  | PSKT_branch
+
+type psk_id =
+  | PSKI_external: id:bytes -> psk_id
+  | PSKI_reinit: group_id:bytes -> epoch:nat -> psk_id
+  | PSKI_branch: group_id:bytes -> epoch:nat -> psk_id
+
+type psk_id_nonce = {
+  id: psk_id;
+  nonce: bytes;
+}
+
+#push-options "--ifuel 1"
+val psk_type_to_network: psk_type -> NT.psk_type_nt
+let psk_type_to_network pt =
+  match pt with
+  | PSKT_external -> NT.PSKT_external
+  | PSKT_reinit -> NT.PSKT_reinit
+  | PSKT_branch -> NT.PSKT_branch
+#pop-options
+
+val network_to_psk_type: NT.psk_type_nt -> result psk_type
+let network_to_psk_type pt =
+  match pt with
+  | NT.PSKT_external -> return PSKT_external
+  | NT.PSKT_reinit -> return PSKT_reinit
+  | NT.PSKT_branch -> return PSKT_branch
+  | _ -> error "network_to_psk_type: invalid psk type"
+
+#push-options "--ifuel 1"
+val psk_id_nonce_to_network: psk_id_nonce -> result NT.pre_shared_key_id_nt
+let psk_id_nonce_to_network psk =
+  if not (Seq.length psk.nonce < 256) then
+    error "psk_to_network: nonce is too long"
+  else (
+    match psk.id with
+    | PSKI_external id -> (
+      if not (Seq.length id < 256) then
+        error "psk_to_network: id is too long"
+      else
+        return (NT.PSKI_external id psk.nonce)
+    )
+    | PSKI_reinit group_id epoch ->
+      if not (Seq.length group_id < 256) then
+        error "psk_to_network: group_id is too long"
+      else if not (epoch < pow2 64) then
+        error "psk_to_network: epoch is too big"
+      else
+        return (NT.PSKI_reinit group_id (Lib.IntTypes.u64 epoch) psk.nonce)
+    | PSKI_branch group_id epoch ->
+      if not (Seq.length group_id < 256) then
+        error "psk_to_network: group_id is too long"
+      else if not (epoch < pow2 64) then
+        error "psk_to_network: epoch is too big"
+      else
+        return (NT.PSKI_branch group_id (Lib.IntTypes.u64 epoch) psk.nonce)
+  )
+#pop-options
+
+val network_to_psk_id_nonce: NT.pre_shared_key_id_nt -> result psk_id_nonce
+let network_to_psk_id_nonce psk_id =
+  match psk_id with
+  | NT.PSKI_external id nonce -> return ({id = PSKI_external id; nonce = nonce})
+  | NT.PSKI_reinit group_id epoch nonce -> return ({id = PSKI_reinit group_id (Lib.IntTypes.v epoch); nonce = nonce})
+  | NT.PSKI_branch group_id epoch nonce -> return ({id = PSKI_reinit group_id (Lib.IntTypes.v epoch); nonce = nonce})
+  | _ -> error "network_to_psk: invalid psk type"
+
+
+type psk_label = {
+  id_nonce: psk_id_nonce;
+  index: nat;
+  count: nat;
+}
+
+val psk_label_to_network: psk_label -> result NT.psk_label_nt
+let psk_label_to_network label =
+  if not (label.count < pow2 16) then
+    error "psk_label_to_network: count is too big"
+  else if not (label.index < pow2 16) then
+    internal_failure "psk_label_to_network: index is too big"
+  else (
+    id <-- psk_id_nonce_to_network label.id_nonce;
+    return ({
+      NT.id = id;
+      NT.index = Lib.IntTypes.u16 label.index;
+      NT.count = Lib.IntTypes.u16 label.count;
+    })
+  )
+
+val network_to_psk_label: NT.psk_label_nt -> result psk_label
+let network_to_psk_label label =
+  id_nonce <-- network_to_psk_id_nonce label.NT.id;
+  return ({
+    id_nonce = id_nonce;
+    index = Lib.IntTypes.v label.NT.index;
+    count = Lib.IntTypes.v label.NT.count;
+  })
+
+// Compute psk_secret[i+1] given psk[i], psk_label[i] and psk_secret[i]
+val compute_psk_secret_step: ciphersuite -> psk_label -> bytes -> bytes -> result bytes
+let compute_psk_secret_step cs label psk prev_psk_secret =
+    label_network <-- psk_label_to_network label;
+    psk_extracted <-- kdf_extract cs (zero_vector cs) psk;
+    psk_input <-- expand_with_label cs psk_extracted (string_to_bytes "derived psk") (NT.ps_psk_label.serialize label_network) (kdf_length cs);
+    new_psk_secret <-- kdf_extract cs psk_input prev_psk_secret;
+    return (new_psk_secret <: bytes)
+
+// Compute psk_secret[n] given psk_secret[ind]
+val compute_psk_secret_aux: ciphersuite -> l:list (psk_id_nonce & bytes) -> ind:nat{ind <= List.Tot.length l} -> bytes -> Tot (result bytes) (decreases (List.Tot.length l - ind))
+let rec compute_psk_secret_aux cs l ind psk_secret_ind =
+  if ind = List.Tot.length l then
+    return psk_secret_ind
+  else (
+    let (id_nonce, psk) = List.Tot.index l ind in
+    let label = ({
+      id_nonce = id_nonce;
+      index = ind;
+      count = List.Tot.length l;
+    }) in
+    next_psk_secret <-- compute_psk_secret_step cs label psk psk_secret_ind;
+    compute_psk_secret_aux cs l (ind+1) next_psk_secret
+  )
+
+val compute_psk_secret: ciphersuite -> list (psk_id_nonce & bytes) -> result bytes
+let compute_psk_secret cs l =
+  compute_psk_secret_aux cs l 0 (zero_vector cs)
